theories/Lang/Maps.v
@@ -1,0 +1,101 @@
+
+From Coq Require Import
+  Nat
+  Strings.String.
+
+From ExtLib Require Import
+  Structures.Maps
+  Data.Map.FMapAList
+  Data.String.
+
+From TICL Require Import Utils.
+
+Module Ctx.
+  Definition Ctx := alist string nat.
+
+  Definition assert1 c (m: Ctx) (p: nat -> Prop) :=
+    exists v, lookup c m = Some v /\ p v.
+
+  Definition assert2 c1 c2 (m: Ctx) (r: nat -> nat -> Prop) :=
+    exists v1 v2, lookup c1 m = Some v1 /\ lookup c2 m = Some v2 /\ r v1 v2.
+
+  (*| Map equations |*)
+  Lemma lookup_add_eq: forall c (v: nat) m,
+    lookup c (add c v m) = Some v.
+  Proof with auto.
+    intros.  
+    pose proof (mapsto_add_eq (R:=@eq string) (V:=nat) m c v).
+    now apply mapsto_lookup in H.
+  Qed.
+
+  Lemma lookup_add_neq: forall c r (v: nat) m,
+    r <> c ->
+    lookup c (add r v m) = lookup c m.
+  Proof with auto.
+    intros.
+    destruct (lookup c (add r v m)) eqn:Hc;
+      destruct (lookup c m) eqn: Hr; rewrite ?mapsto_lookup in *.
+    - apply mapsto_add_neq with (R:=eq) in Hc...
+      rewrite <- mapsto_lookup in *.
+      rewrite Hc in Hr; inv Hr...
+    - apply mapsto_add_neq with (R:=eq) in Hc...
+      rewrite <- mapsto_lookup in Hc.
+      rewrite Hc in Hr; inv Hr.
+    - rewrite mapsto_add_neq with (R:=eq) in Hr. 
+      rewrite <- mapsto_lookup in Hr.
+      rewrite Hc in Hr; inv Hr.
+      apply H.
+    - reflexivity.
+      Unshelve.
+      exact eq.
+      typeclasses eauto.
+      typeclasses eauto.
+      typeclasses eauto.
+      typeclasses eauto.
+  Qed.
+
+  Lemma assert1_add_eq: forall c (v: nat) m p,
+      p v ->
+      assert1 c (add c v m) p.
+  Proof with eauto.
+    intros.
+    unfold assert1.
+    pose proof (mapsto_add_eq (R:=@eq string) (V:=nat) m c v).
+    apply mapsto_lookup in H0.
+    rewrite H0...
+  Qed.
+
+  Lemma assert1_add_neq: forall c1 c2 (v: nat) m p,
+      assert1 c1 m p ->
+      c1 <> c2 ->
+      assert1 c1 (add c2 v m) p.
+  Proof with eauto.
+    intros.
+    unfold assert1 in *.
+    destruct H as (v1 & Hc1 & Hv1).    
+    exists v1; split...
+    rewrite mapsto_lookup with (R:=@eq string) in Hc1 |- *.
+    apply mapsto_add_neq with (R:=@eq string)...
+    Unshelve.
+    typeclasses eauto.
+  Qed.
+  
+  Lemma assert2_add_l: forall c1 c2 (v1 v2: nat) m p,
+      c1 <> c2 ->
+      p v1 v2 ->
+      assert2 c1 c2 (add c1 v1 (add c2 v2 m)) p.
+  Proof with eauto.
+    intros.
+    unfold assert2.
+    pose proof (mapsto_add_eq (R:=@eq string) (V:=nat) (add c2 v2 m) c1 v1) as H1.
+    apply mapsto_lookup in H1.
+    assert (H2: lookup c2 (add c1 v1 (add c2 v2 m)) = Some v2).
+    - rewrite mapsto_lookup with (R:=eq).
+      apply mapsto_add_neq...
+      apply mapsto_add_eq.
+    - exists v1, v2.
+      rewrite H1, H2...
+      Unshelve.
+      typeclasses eauto.
+  Qed.
+End Ctx.
